Tue May 21 21:09:48 DST 2019

UntypedArith.v
@@ -1,7 +1,4 @@
-Definition relation (X:Type) := X -> X -> Prop.
-
-Definition normal_form {X:Type} (R:relation X) (t:X) : Prop :=
-~ exists t', R t t'.
+Require Export ReductionSystem.
 
 Inductive term : Type :=
 | tzero : term
