ReductionSystem.v
@@ -1,0 +1,4 @@
+Definition relation (X:Type) := X -> X -> Prop.
+
+Definition normal_form {X:Type} (R:relation X) (t:X) : Prop :=
+~ exists t', R t t'.
